Add freshness and value/value substitution

proof/Exp.v
@@ -24,6 +24,68 @@ Inductive VALUE : exp -> Prop :=
 Hint Constructors VALUE.
 
 
+(* free variables *****************************************)
+Inductive freeX : name -> exp -> Prop :=
+ | FreeX_var
+   : forall n, freeX n (XVar n)
+
+ | FreeX_lam
+   :  forall x y T11 t12
+   ,  y <> x
+   -> freeX x t12
+   -> freeX x (XLam y T11 t12)
+
+ | FreeX_app1
+   :  forall x t1 t2
+   ,  freeX x t1 -> freeX x (XApp t1 t2)
+
+ | FreeX_app2 
+   :  forall x t1 t2
+   ,  freeX x t2 -> freeX x (XApp t1 t2).
+
+Tactic Notation "freeX_cases" tactic(first) ident(c) :=
+  first;
+  [ Case_aux c "FreeX_var"
+  | Case_aux c "FreeX_lam"
+  | Case_aux c "FreeX_app1"
+  | Case_aux c "FreeX_app2"].
+
+Hint Constructors freeX.
+
+Definition closed (t:exp) 
+ := forall x, ~(freeX x t).
+
+
+Lemma nocapture_lam
+ :  forall x y t T
+ ,  freeX x (XLam y T t) -> x <> y.
+Proof.
+ intros.
+ inversion H. subst.
+ unfold not. unfold not in H3. intro. auto.
+Qed.
+
+
+(* freshness **********************************************)
+Inductive freshX : name -> exp -> Prop :=
+ | FreshX_var
+   :  forall n1 n2
+   ,  n1 <> n2 
+   -> freshX n1 (XVar n2)
+
+ | FreshX_lam
+   :  forall n1 n2 T t11
+   ,  n1 <> n2 
+   -> freshX n1 t11 
+   -> freshX n1 (XLam n2 T t11)
+
+ | FreshX_app
+   :  forall n1 t11 t12
+   ,  freshX n1 t11
+   -> freshX n1 t12
+   -> freshX n1 (XApp t11 t12).
+
+
 (* substitution *******************************************)
 (* TODO: only works for s closed *)
 
@@ -33,10 +95,9 @@ Fixpoint subst (n : name) (s : exp) (t : exp) : exp :=
     => if beq_name n n' then s else t
 
     |  XLam n' T x1
-    => XLam n' T 
-         (if beq_name n n'
-              then x1
-              else subst n s x1)
+    => if beq_name n n'
+        then XLam n' T x1
+        else XLam n' T (subst n s x1)  
 
     |  XApp x1 x2 
     => XApp (subst n s x1) (subst n s x2)
