proof/Context.v
@@ -33,14 +33,21 @@ Qed.
 (* Skippin over members that don't match the name we care about *)
 Lemma extend_neq
  :  forall A (ctx: partial_map A) x1 T x2
- ,  beq_name x1 x2 = false
+ ,  x2 <> x1
  -> (extend ctx x2 T) x1 = ctx x1.
 Proof. 
- intros. unfold extend. 
- rewrite beq_name_sym in H. rewrite -> H. tauto.
+ intros. unfold extend.
+ remember (beq_name x2 x1) as e. destruct e.
+ apply true_name_eq in Heqe. subst. tauto. trivial.
 Qed.
 
 
+(* Swap order of elements in context *)
+Lemma extend_swap
+ :   forall A (ctx: partial_map A) x T1 y T2
+ ,   x <> y
+ ->  (extend (extend ctx x T1) y T2) = (extend (extend ctx y T2) x T1).
+Proof. admit. Qed.
 
 
 
