proof/Name.v
@@ -24,17 +24,6 @@ Proof.
 Qed.
 
 
-Theorem beq_name_eq 
- : forall n1 n2
- , true = beq_name n1 n2 -> n1 = n2.
-Proof.
- intros n1 n2. 
- destruct n1. destruct n2.
- unfold beq_name.
- intros eq. apply beq_nat_eq in eq. auto.
-Qed.
-
-
 Theorem beq_name_sym
  : forall n1 n2
  , beq_name n1 n2 = beq_name n2 n1.
@@ -44,4 +33,51 @@ Proof.
  unfold beq_name.
  apply beq_nat_sym.
 Qed.
+
+
+(* bool equality ******************************************)
+Theorem true_name_eq 
+ : forall n1 n2
+ , true = beq_name n1 n2 -> n1 = n2.
+Proof.
+ intros n1 n2. 
+ destruct n1. destruct n2.
+ unfold beq_name.
+ intros eq. apply true_nat_eq in eq. auto.
+Qed.
+
+
+Theorem eq_name_true
+ : forall n1 n2
+ , n1 = n2 -> true = beq_name n1 n2.
+Proof.
+ intros n1 n2.
+ destruct n1. destruct n2.
+ unfold beq_name. intro. inversion H.
+ apply eq_nat_true. auto.
+Qed.
+
+
+Theorem false_name_neq
+ : forall n1 n2
+ , false = beq_name n1 n2 -> n1 <> n2.
+Proof. admit. Qed.
+
+
+Theorem neq_name_false
+ : forall n1 n2
+ , n1 <> n2 -> false = beq_name n1 n2.
+Proof. admit. Qed. 
+
+
+
+
+
+
+
+
+
+
+
+
 
