proof/TyJudge.v
@@ -35,8 +35,119 @@ Hint Unfold  beq_name beq_nat extend.
 Hint Resolve extend_eq. 
 
 
+(* A well typed expression with a free variable
+   has that variable in the type environment.  *)
+Lemma tyenv_contains_free_vars
+ :  forall x t T env
+ ,  freeX x t
+ -> TYPE env t T
+ -> (exists T', env x = some T').
+Proof.
+ intros.
+ generalize dependent env.
+ generalize dependent T.
+ induction H ; intros.
+ Case "XVar".
+  inversion H0. subst.
+  exists T. assumption.
+ Case "XLam".
+  inversion H1. subst.
+  apply IHfreeX in H7. 
+  rewrite extend_neq in H7. auto.
+  assumption.
+ Case "XApp/app1". 
+  inversion H0. subst.
+  eapply IHfreeX. apply H4.
+ Case "XApp/app2".
+  inversion H0. subst.
+  eapply IHfreeX. apply H6.
+Qed.
 
 
+(* We can ignore elements of the type environment if that
+   variable is not free in the expresison being checked. *)
+Lemma tyenv_invariance 
+ : forall env env' t T
+ ,  TYPE env t T
+ -> (forall x, freeX x t -> env x = env' x)
+ -> TYPE env' t T.
+Proof.
+ intros.
+ generalize dependent env'.
+ induction H; intros.
+ Case "XVar".
+  apply TYVar.
+  rewrite <- H0.
+  assumption. auto.
+ Case "XLam".
+  apply TYLam.
+  eapply IHTYPE.
+  intros.
+  unfold extend.
+  remember (beq_name x x0) as e. destruct e.
+  trivial.
+  eapply H0.
+  eapply FreeX_lam.
+  apply false_name_neq. assumption. assumption.
+ Case "XApp".
+  eapply TYApp. eauto. eauto.
+Qed.
 
 
- 
+(* TODO: The freshX predicate requires z not to appear
+         at all in t1. Weaken just to avoid capture by lambda
+         in t1.
+*)
+Lemma subst_value_value
+ :  forall env x val t1 T1 T2
+ ,  (forall z, freeX z val -> freshX z t1)
+ -> TYPE (extend env x T2) t1  T1
+ -> TYPE env               val T2
+ -> TYPE env  (subst x val t1) T1.
+Proof.
+ intros env x val t1 T1 T2.
+ generalize dependent env.
+ generalize dependent T1.
+ induction t1.
+ Case "XVar".
+  intros. simpl. rename n into y.
+  remember (beq_name x y) as e. destruct e.
+  SCase "x=y".
+   apply true_name_eq in Heqe. subst.
+   inversion H0. subst.
+   rewrite extend_eq in H4. inversion H4. subst. assumption.
+  SCase "x<>y".
+   apply TYVar.
+   inversion H0. subst.
+   apply false_name_neq in Heqe.
+   rewrite extend_neq in H4. assumption. assumption.
+ Case "XLam".
+  intros. rename n into y.
+  simpl. remember (beq_name x y) as e. destruct e.
+  SCase "x=y".
+   apply true_name_eq in Heqe. subst.
+   eapply tyenv_invariance. eauto.
+   intros. apply extend_neq.
+   apply nocapture_lam in H2.
+   apply sym_not_equal in H2. assumption.
+  SCase "x<>y".
+   apply false_name_neq in Heqe.
+   inversion H0. subst.
+   apply TYLam. apply IHt1. 
+   intros. apply H in H2. inversion H2. subst. assumption.
+   rewrite extend_swap. assumption.
+   apply sym_not_equal. assumption.
+   eapply tyenv_invariance. eauto.
+   intros. apply H in H2. inversion H2. subst.
+   rewrite -> extend_neq. trivial.
+   apply sym_not_equal. assumption.
+ Case "XApp".
+   intros. simpl.
+   inversion H0. subst.
+   eapply TYApp.
+   eapply IHt1_1 in H5. apply H5. 
+    intros. apply H in H2. inversion H2. auto. assumption.
+   eapply IHt1_2 in H7. apply H7.
+    intros. apply H in H2. inversion H2. auto. assumption.
+Qed.
+
